pcuic/theories/PCUICCumulProp.v
@@ -365,11 +365,11 @@ Proof.
   intros x y; unfold eq_univ_prop; intuition.
 Qed.
 
-Lemma UnivExprSet_For_all (P : UnivExpr.t -> Prop) (u : AlgebraicExpr.t) :
-  UnivExprSet.For_all P u <->
-  Forall P (UnivExprSet.elements u).
+Lemma LevelExprSet_For_all (P : LevelExpr.t -> Prop) (u : LevelAlgExpr.t) :
+  LevelExprSet.For_all P u <->
+  Forall P (LevelExprSet.elements u).
 Proof.
-  rewrite NonEmptySetFacts.UnivExprSet_For_all_exprs.
+  rewrite NonEmptySetFacts.LevelExprSet_For_all_exprs.
   pose proof (NonEmptySetFacts.to_nonempty_list_spec u).
   destruct (NonEmptySetFacts.to_nonempty_list u). rewrite -H. simpl.
   split. constructor; intuition.
@@ -377,30 +377,30 @@ Proof.
 Qed.
 
 Lemma univ_expr_set_in_elements e s : 
-  UnivExprSet.In e s <-> In e (UnivExprSet.elements s).
+  LevelExprSet.In e s <-> In e (LevelExprSet.elements s).
 Proof.
-  rewrite -UnivExprSet.elements_spec1. generalize (UnivExprSet.elements s).
+  rewrite -LevelExprSet.elements_spec1. generalize (LevelExprSet.elements s).
   now eapply InA_In_eq.
 Qed.
 
-Lemma univ_epxrs_elements_map g s : 
-  forall e, In e (UnivExprSet.elements (NonEmptySetFacts.map g s)) <->
-      In e (map g (UnivExprSet.elements s)).
+Lemma univ_epxrs_elements_map g s :
+  forall e, In e (LevelExprSet.elements (NonEmptySetFacts.map g s)) <->
+      In e (map g (LevelExprSet.elements s)).
 Proof.
   intros e.
   unfold NonEmptySetFacts.map.
   pose proof (NonEmptySetFacts.to_nonempty_list_spec s).
   destruct (NonEmptySetFacts.to_nonempty_list s) as [e' l] eqn:eq.  
   rewrite -univ_expr_set_in_elements NonEmptySetFacts.add_list_spec.
-  rewrite -H. simpl. rewrite UnivExprSet.singleton_spec.
+  rewrite -H. simpl. rewrite LevelExprSet.singleton_spec.
   intuition auto.
 Qed.
   
-Lemma Forall_elements_in P s : Forall P (UnivExprSet.elements s) <-> 
-  (forall x, UnivExprSet.In x s -> P x).
+Lemma Forall_elements_in P s : Forall P (LevelExprSet.elements s) <->
+  (forall x, LevelExprSet.In x s -> P x).
 Proof.
   setoid_rewrite univ_expr_set_in_elements.
-  generalize (UnivExprSet.elements s).
+  generalize (LevelExprSet.elements s).
   intros.
   split; intros.
   induction H; depelim H0; subst => //; auto.
@@ -410,8 +410,8 @@ Proof.
 Qed.
 
 Lemma univ_exprs_map_all P g s : 
-  Forall P (UnivExprSet.elements (NonEmptySetFacts.map g s)) <->
-  Forall (fun x => P (g x)) (UnivExprSet.elements s).
+  Forall P (LevelExprSet.elements (NonEmptySetFacts.map g s)) <->
+  Forall (fun x => P (g x)) (LevelExprSet.elements s).
 Proof.
   rewrite !Forall_elements_in.
   setoid_rewrite NonEmptySetFacts.map_spec.
@@ -421,10 +421,10 @@ Proof.
 Qed.
 
 Lemma expr_set_forall_map f g s : 
-  UnivExprSet.for_all f (NonEmptySetFacts.map g s) <->
-  UnivExprSet.for_all (fun e => f (g e)) s.
+  LevelExprSet.for_all f (NonEmptySetFacts.map g s) <->
+  LevelExprSet.for_all (fun e => f (g e)) s.
 Proof.
-  rewrite /is_true !UnivExprSet.for_all_spec !UnivExprSet_For_all.
+  rewrite /is_true !LevelExprSet.for_all_spec !LevelExprSet_For_all.
   apply univ_exprs_map_all.
 Qed.
 
@@ -435,7 +435,7 @@ Qed.
 
 (* Lemma is_prop_subst_level_expr u1 u2 s : 
   Forall2 (fun x y : Level.t => eq_univ_prop (Universe.make x) (Universe.make y)) u1 u2  ->
-  UnivExpr.is_prop (subst_instance_level_expr u1 s) = UnivExpr.is_prop (subst_instance_level_expr u2 s).
+  LevelExpr.is_prop (subst_instance_level_expr u1 s) = LevelExpr.is_prop (subst_instance_level_expr u2 s).
 Proof.
   intros hu. destruct s; simpl; auto.
   destruct e as [[] ?]; simpl; auto.
